first working version of ecrecover

c/keccak.c
@@ -1,0 +1,154 @@
+#include <string.h>
+#include "keccak.h"
+
+#if defined(_MSC_VER)
+#define SHA3_CONST(x) x
+#else
+#define SHA3_CONST(x) x##L
+#endif
+
+#ifndef SHA3_ROTL64
+#define SHA3_ROTL64(x, y) \
+	(((x) << (y)) | ((x) >> (64 - (y))))
+#endif
+
+static const uint64_t keccakf_rndc[24] = {
+    SHA3_CONST(0x0000000000000001UL), SHA3_CONST(0x0000000000008082UL),
+    SHA3_CONST(0x800000000000808aUL), SHA3_CONST(0x8000000080008000UL),
+    SHA3_CONST(0x000000000000808bUL), SHA3_CONST(0x0000000080000001UL),
+    SHA3_CONST(0x8000000080008081UL), SHA3_CONST(0x8000000000008009UL),
+    SHA3_CONST(0x000000000000008aUL), SHA3_CONST(0x0000000000000088UL),
+    SHA3_CONST(0x0000000080008009UL), SHA3_CONST(0x000000008000000aUL),
+    SHA3_CONST(0x000000008000808bUL), SHA3_CONST(0x800000000000008bUL),
+    SHA3_CONST(0x8000000000008089UL), SHA3_CONST(0x8000000000008003UL),
+    SHA3_CONST(0x8000000000008002UL), SHA3_CONST(0x8000000000000080UL),
+    SHA3_CONST(0x000000000000800aUL), SHA3_CONST(0x800000008000000aUL),
+    SHA3_CONST(0x8000000080008081UL), SHA3_CONST(0x8000000000008080UL),
+    SHA3_CONST(0x0000000080000001UL), SHA3_CONST(0x8000000080008008UL)
+};
+
+static const unsigned keccakf_rotc[24] = {
+  1, 3, 6, 10, 15, 21, 28, 36, 45, 55, 2, 14, 
+  27, 41, 56, 8, 25, 43, 62, 18, 39, 61, 20, 44
+};
+
+static const unsigned keccakf_piln[24] = {
+  10, 7, 11, 17, 18, 3, 5, 16, 8, 21, 24, 4, 
+  15, 23, 19, 13, 12, 2, 20, 14, 22, 9, 6, 1
+};
+
+static void keccakf(uint64_t s[25])
+{
+  int i, j, round;
+  uint64_t t, bc[5];
+  #define KECCAK_ROUNDS 24
+
+  for(round = 0; round < KECCAK_ROUNDS; round++) 
+  {
+    /* Theta */
+    for(i = 0; i < 5; i++)
+      bc[i] = s[i] ^ s[i + 5] ^ s[i + 10] ^ s[i + 15] ^ s[i + 20];
+
+    for(i = 0; i < 5; i++) 
+    {
+      t = bc[(i + 4) % 5] ^ SHA3_ROTL64(bc[(i + 1) % 5], 1);
+      for(j = 0; j < 25; j += 5)
+        s[j + i] ^= t;
+    }
+
+    /* Rho Pi */
+    t = s[1];
+    for(i = 0; i < 24; i++) 
+    {
+      j = keccakf_piln[i];
+      bc[0] = s[j];
+      s[j] = SHA3_ROTL64(t, keccakf_rotc[i]);
+      t = bc[0];
+    }
+    
+    /* Chi */
+    for(j = 0; j < 25; j += 5) {
+      for(i = 0; i < 5; i++)
+        bc[i] = s[j + i];
+      for(i = 0; i < 5; i++)
+        s[j + i] ^= (~bc[(i + 1) % 5]) & bc[(i + 2) % 5];
+    }
+
+    /* Iota */
+    s[0] ^= keccakf_rndc[round];
+  }
+}
+
+void sha3_Update(void *priv, void const *bufIn, size_t len)
+{
+  sha3_context *ctx = (sha3_context *) priv;
+  size_t words = len / 8;
+  unsigned tail = len - (len / 8) * 8;
+  size_t i;
+  const uint8_t *buf = bufIn;
+
+  for(i = 0; i < words; i++, buf += 8) 
+  {
+    const uint64_t t = (uint64_t) (buf[0]) |
+            ((uint64_t) (buf[1]) << 8 * 1) |
+            ((uint64_t) (buf[2]) << 8 * 2) |
+            ((uint64_t) (buf[3]) << 8 * 3) |
+            ((uint64_t) (buf[4]) << 8 * 4) |
+            ((uint64_t) (buf[5]) << 8 * 5) |
+            ((uint64_t) (buf[6]) << 8 * 6) |
+            ((uint64_t) (buf[7]) << 8 * 7);
+    ctx->u.s[ctx->wordIndex] ^= t;
+    if(++ctx->wordIndex == 17) 
+    {
+      keccakf(ctx->u.s);
+      ctx->wordIndex = 0;
+    }
+  }
+
+  while (tail--) {
+    ctx->saved |= (uint64_t) (*(buf++)) << ((ctx->byteIndex++) * 8);
+  }
+}
+
+void const * sha3_Finalize(void *priv)
+{
+  sha3_context *ctx = (sha3_context *) priv;
+  uint64_t t = (uint64_t)(((uint64_t) 1) << (ctx->byteIndex * 8));
+  unsigned i;
+
+  ctx->u.s[ctx->wordIndex] ^= ctx->saved ^ t;
+  ctx->u.s[16] ^= SHA3_CONST(0x8000000000000000UL);
+  keccakf(ctx->u.s);
+
+  for(i = 0; i < 25; i++) 
+  {
+    const unsigned t1 = (uint32_t) ctx->u.s[i];
+    const unsigned t2 = (uint32_t) ((ctx->u.s[i] >> 16) >> 16);
+    ctx->u.sb[i * 8 + 0] = (uint8_t) (t1);
+    ctx->u.sb[i * 8 + 1] = (uint8_t) (t1 >> 8);
+    ctx->u.sb[i * 8 + 2] = (uint8_t) (t1 >> 16);
+    ctx->u.sb[i * 8 + 3] = (uint8_t) (t1 >> 24);
+    ctx->u.sb[i * 8 + 4] = (uint8_t) (t2);
+    ctx->u.sb[i * 8 + 5] = (uint8_t) (t2 >> 8);
+    ctx->u.sb[i * 8 + 6] = (uint8_t) (t2 >> 16);
+    ctx->u.sb[i * 8 + 7] = (uint8_t) (t2 >> 24);
+  }
+
+  return (ctx->u.sb);
+}
+
+bytes32 keccak(void* p, size_t input_len) 
+{
+  unsigned i;
+  sha3_context c;
+  const uint8_t *hash;
+  bytes32 bs;
+
+  memset(&c, 0, sizeof(c));
+  c.capacityWords = 0x80000008; 
+  sha3_Update(&c, p, input_len);
+  hash = sha3_Finalize(&c);
+
+  memcpy(bs.data, hash, 32);
+  return bs;
+}
