c/keccak.h
@@ -1,0 +1,27 @@
+#include <stdint.h>
+
+typedef struct {
+    uint64_t saved;             /* the portion of the input message that we
+                                 * didn't consume yet */
+    union {                     /* Keccak's state */
+        uint64_t s[25];
+        uint8_t sb[25 * 8];
+    } u;
+    unsigned byteIndex;         /* 0..7--the next byte after the set one
+                                 * (starts from 0; 0--none are buffered) */
+    unsigned wordIndex;         /* 0..24--the next word to integrate input
+                                 * (starts from 0) */
+    unsigned capacityWords;     /* the double size of the hash output in
+                                 * words (e.g. 16 for Keccak 512) */
+} sha3_context;
+
+// void sha3_Update(void *priv, void const *bufIn, size_t len);
+// 
+// void const *sha3_Finalize(void *priv);
+
+typedef struct 
+{
+  uint8_t data[32];
+} bytes32;
+
+bytes32 keccak(void* p, size_t input_len);
