Blanc.lean
@@ -5,10 +5,175 @@ partial def Bytes.chunks (bs : Bytes) : List Bytes :=
   | (_, []) => [bs]
   | (bs', bs'') => bs' :: chunks bs''
 
+def Bytes.toHexLine (bs : Bytes) : String :=
+  s!"hex\"{bs.toHextring}\""
+
 def WethByteCode : String :=
   List.foldr
      (λ s0 s1 => s0 ++ "\n" ++ s1)
-     "" <| List.map Bytes.toHexString
-        <| Bytes.chunks <| Option.getD weth'.compile []
+     "" <| List.map Bytes.toHexLine
+        <| Bytes.chunks <| Option.getD weth.compile []
 
-def main : IO Unit := IO.println WethByteCode
+-- def main : IO Unit := IO.println WethByteCode
+
+--mutual
+--  inductive RLP : Type
+--    | bytes : Bytes → RLP
+--    | list : RLPs → RLP
+--  inductive RLPs : Type
+--    | nil : RLPs
+--    | cons : RLP → RLPs → RLPs
+--end
+--
+--#exit
+inductive RLP : Type
+  | bytes : Bytes → RLP
+  | list : List RLP → RLP
+
+def List.splitAt? {ξ : Type u} : Nat → List ξ → Option (List ξ × List ξ)
+  | 0, xs => some ([], xs)
+  | _ + 1, [] => none
+  | n + 1, x :: xs => .map (x :: ·) id <$> xs.splitAt? n
+
+
+def Bytes.toNat' : Nat → Bytes → Nat
+  | k, [] => k
+  | k, b :: bs => Bytes.toNat' ((k * 256) + b.toNat) bs
+
+def Bytes.toNat (bs : Bytes) : Nat := bs.toNat' 0
+
+
+def Nat.toBytes' (n : Nat) : Bytes :=
+  if n < 256
+  then [n.toByte]
+  else (n % 256).toByte :: (n / 256).toBytes'
+
+def Nat.toBytes (n : Nat) : Bytes := n.toBytes'.reverse
+
+mutual
+  def RLP.decode' : Nat → Bytes → Option (RLP × Bytes)
+    | _, [] => none
+    | 0, _ :: _ => none
+    | _ + 1, b@⦃0, _, _, _, _, _, _, _⦄ :: bs => some (.bytes [b], bs)
+    | _ + 1, b@⦃1, 0, 1, 1, 1, _, _, _⦄ :: bs => do
+      let (lbs, bs') ← List.splitAt? (b - Ox xB x7).toNat bs
+      let (rbs, bs'') ← List.splitAt? (Bytes.toNat lbs) bs'
+      return ⟨.bytes rbs, bs''⟩
+    | _ + 1, b@⦃1, 0, _, _, _, _, _, _⦄ :: bs =>
+      .map .bytes id <$> List.splitAt? (b - Ox x8 x0).toNat bs
+    | k + 1, b@⦃1, 1, 1, 1, 1, _, _, _⦄ :: bs => do
+      let (lbs, bs') ← List.splitAt? (b - Ox xF x7).toNat bs
+      let (rbs, bs'') ← List.splitAt? (Bytes.toNat lbs) bs'
+      let rs ← RLPs.decode k rbs
+      return ⟨.list rs, bs''⟩
+    | k + 1, b@⦃1, 1, _, _, _, _, _, _⦄ :: bs => do
+      let (rbs, bs') ← List.splitAt? (b - Ox xC x0).toNat bs
+      let rs ← RLPs.decode k rbs
+      return ⟨.list rs, bs'⟩
+  def RLPs.decode : Nat → Bytes → Option (List RLP)
+    | _, [] => some []
+    | 0, _ :: _ => none
+    | k + 1, bs@(_ :: _) => do
+      let (r, bs') ← RLP.decode' (k + 1) bs
+      let rs ← RLPs.decode k bs'
+      return (r :: rs)
+end
+
+def RLP.decode (bs : Bytes) : Option RLP :=
+  match RLP.decode' bs.length bs with
+  | some (r, []) => some r
+  | _ => none
+
+def RLP.encodeBytes : Bytes → Bytes
+  | [b] =>
+    if b < (Ox x8 x0)
+    then [b]
+    else [Ox x8 x1, b]
+  | bs =>
+    if bs.length < 56
+    then (Ox x8 x0 + bs.length.toByte) :: bs
+    else let lbs : Bytes := bs.length.toBytes
+         (Ox xB x7 + lbs.length.toByte) :: (lbs ++ bs)
+
+mutual
+  def RLP.encode : RLP → Bytes
+    | .bytes [b] =>
+      if b < (Ox x8 x0)
+      then [b]
+      else [Ox x8 x1, b]
+    | .bytes bs =>
+      if bs.length < 56
+      then (Ox x8 x0 + bs.length.toByte) :: bs
+      else let lbs : Bytes := bs.length.toBytes
+           (Ox xB x7 + lbs.length.toByte) :: (lbs ++ bs)
+    | .list rs => RLPs.encode rs
+  def RLPs.encodeMap : List RLP → Bytes
+    | .nil => []
+    | .cons r rs => r.encode ++ RLPs.encodeMap rs
+  def RLPs.encode (rs : List RLP) : Bytes :=
+    let bs := RLPs.encodeMap rs
+    let len := bs.length
+    if len < 56
+    then (Ox xC x0 + len.toByte) :: bs
+    else let lbs : Bytes := len.toBytes
+         (Ox xF x7 + lbs.length.toByte) :: (lbs ++ bs)
+end
+
+partial def RLP.toStrings : RLP → List String
+  | .bytes bs => [s!"0x{bs.toHextring}"]
+  | .list rs => "List:" :: (rs.map RLP.toStrings).flatten.map ("  " ++ ·)
+
+def Strings.join : List String → String
+  | [] => ""
+  | s :: ss => s ++ "\n" ++ Strings.join ss
+
+def Hexes.toBytes : List Hex → Option Bytes
+  | [] => some []
+  | [_] => none
+  | h0 :: h1 :: hs => (Ox h0 h1 :: ·) <$> Hexes.toBytes hs
+
+def Hextring.toBytes (s : String) : Option Bytes :=
+  Hexes.toBytes <| s.data.map Hexar.toHex
+
+def notTxBytes : Bytes :=
+  (Hextring.toBytes "f885800a8404c4b40094cccccccccccccccccccccccccccccccccccccccc01a4693c613900000000000000000000000000000000000000000000000000000000000000001ba0e8ff56322287185f6afd3422a825b47bf5c1a4ccf0dc0389cdc03f7c1c32b7eaa0776b02f9f5773238d3ff36b74a123f409cd6420908d7855bbe4c8ff63e00d698").getD []
+
+def highValueTxBytes : Bytes :=
+  (Hextring.toBytes "f87f800182520894095e7baea6a6c7c4c2dfeb977efac326af552d87a0ffffffffffffffffffffffffffffffffffffffffffffffffffffffffffffffff801ba048b55bfa915ac795c431978d8a6a992b628d557da5ff759b307d495a36649353a01fffd310ac743f371de3b9f7f9cb56c0b28ad43601b4ab949f53faa07bd2c804").getD []
+
+def optionToIO {ξ} (o : Option ξ) : IO ξ := do
+  match o with
+  | none => throw (IO.Error.userError "none value")
+  | some x => pure x
+
+@[extern "ecrecover"]
+opaque ecrecover : ByteArray → ByteArray → ByteArray
+
+def Byte.toUInt8 (b : Byte) : UInt8 := ⟨⟨b.toNat, b.toNat_lt_pow⟩⟩
+def UInt8.toByte (i : UInt8) : Byte := i.toBitVec.toFin.val.toByte
+
+def Bytes.toBytesArray (bs : Bytes) : ByteArray := ⟨⟨List.map Byte.toUInt8 bs⟩⟩
+def ByteArray.toBytes (a : ByteArray) : Bytes := a.data.toList.map UInt8.toByte
+
+def main : IO Unit := do
+  let bs := highValueTxBytes
+  let (RLP.list [txType, nonce, gasPrice, toAddr, val, calldata, .bytes v, .bytes r, .bytes s])
+    ← (optionToIO <| RLP.decode bs)
+    | throw (IO.Error.userError "Error : decoded list length ≠ 9")
+  let bs' := RLP.encode <| .list [txType, nonce, gasPrice, toAddr, val, calldata]
+  let hs := bs'.keccak
+
+  IO.println <| s!"v : {v.toNat}"
+  IO.println <| s!"r : {r.toHextring}"
+  IO.println <| s!"s : {s.toHextring}"
+  IO.println <| s!"Hash of txdata excluding signature: {Bits.toHextring 32 hs}"
+
+  let rsa : ByteArray := Bytes.toBytesArray (r ++ s)
+  let hsa : ByteArray := Bytes.toBytesArray (@Bits.toBytes 32 hs)
+
+  match (ecrecover rsa hsa).toBytes with
+  | [] => IO.println "Unreachable code : ecrecover should never return empty bytes"
+  | b :: pa =>
+    if b = 0
+    then IO.println "ecrecover failed"
+    else IO.println <| s!"Recovered public address : {Bytes.toHextring pa}"
